Verified RunningExample.
Co-authored-by: Copilot <223556219+Copilot@users.noreply.github.com>

seiostar/RunningExample.fst
@@ -1,6 +1,7 @@
 module RunningExample
 
 open FStar.Tactics.V1
+open FStar.Classical
 open Trace
 open IOStar
 open RQ.Metaprogram
@@ -94,7 +95,7 @@ let openfile_spec (f : string) =
     (fun h -> True)
     (fun h lt (r:resexn file_descr) ->
       Inl? r ==>
-      exists fd. lt == [ EvOpen f (Inl fd) ]
+      lt == [ EvOpen f (Inl (Inl?.v r)) ]
     )
 
 let openfile_sat_spec f :
@@ -107,7 +108,7 @@ let read_spec (fd : file_descr) =
     (fun h -> True)
     (fun h lt (r:resexn string) ->
       Inl? r ==>
-      exists fd. lt == [ EvRead fd (Inl (Inl?.v r)) ]
+      lt == [ EvRead fd (Inl (Inl?.v r)) ]
     )
 
 let read_sat_spec fd :
@@ -120,7 +121,7 @@ let close_spec (fd : file_descr) =
     (fun h -> True)
     (fun h lt (r:resexn unit) ->
       Inl? r ==>
-      exists fd. lt == [ EvClose fd (Inl ()) ]
+      lt == [ EvClose fd (Inl ()) ]
     )
 
 let close_sat_spec fd :
@@ -148,6 +149,7 @@ let hist_bind_commut_resexn #a #b (m : hist (resexn a)) (k : a -> io (resexn b))
   end ;
   lem_hist_bind_equiv m m (fun (r : resexn a) -> theta (match r with | Inl x -> k x | Inr x -> io_return (Inr x))) (fun r -> match r with | Inl x -> theta (k x) | Inr x -> hist_return (Inr x))
 
+unfold
 let hist_inl #a #b (k : a -> hist (resexn b)) (r : resexn a) : hist (resexn b) =
   fun h p ->
     (Inl? r ==> k (Inl?.v r) h p) /\
@@ -165,6 +167,127 @@ let hist_bind_resexn_weaken #a #b (m : hist (resexn a)) (k : a -> io (resexn b))
     | Inr x -> theta_monad_morphism_ret #(resexn b) (Inr x)
   end ;
   lem_hist_bind_subset m m (fun (r : resexn a) -> theta (match r with | Inl x -> k x | Inr x -> io_return (Inr x))) (hist_inl (fun x -> theta (k x)))
+
+let lem_hist_bind_hist_inl_subset #a #b (w:hist (resexn a)) (k1 k2 : a -> hist (resexn b))
+  (lem : (x:a -> Lemma (k1 x ⊑ k2 x))) :
+  Lemma (hist_bind w (hist_inl k1) ⊑ hist_bind w (hist_inl k2))
+= Classical.forall_intro (Classical.move_requires lem)
+
+let lem_hist_bind_match_resexn_subset (#a #b:Type) (m:hist (resexn a))
+  (k1 k2 : a -> hist (resexn b))
+  (lem : (x:a -> Lemma (k1 x ⊑ k2 x))) :
+  Lemma (
+    hist_bind m (fun res -> match res with | Inl x -> k1 x | Inr e -> hist_return (Inr e))
+    ⊑
+    hist_bind m (fun res -> match res with | Inl x -> k2 x | Inr e -> hist_return (Inr e))
+  )
+= Classical.forall_intro (Classical.move_requires lem)
+
+#push-options "--z3rlimit 50"
+let close_return_pointwise (fd:file_descr) (r:string) (res:resexn unit) :
+  Lemma (
+    theta (match res with | Inl () -> io_return (Inl r) | Inr x -> io_return (Inr x))
+    ⊑
+    (hist_inl (fun () -> hist_return (Inl r))) res
+  )
+= theta_monad_morphism_ret (Inl #string #unit r);
+  theta_monad_morphism_ret (Inr #string #unit ());
+  match res with | Inl () -> () | Inr _ -> ()
+#pop-options
+
+#push-options "--z3rlimit 50"
+let close_return_sat_spec (fd:file_descr) (r:string) :
+  Lemma (
+    theta (let!@! () = io_call OClose fd in io_return (Inl r))
+    ⊑
+    hist_bind (close_spec fd) (hist_inl (fun () -> hist_return (Inl r)))
+  )
+= calc (⊑) {
+    theta (let!@! () = io_call OClose fd in io_return (Inl r)) ;
+    `hist_equiv` {
+      theta_monad_morphism_bind (io_call OClose fd) (fun res ->
+        match res with | Inl () -> io_return (Inl r) | Inr x -> io_return (Inr x))
+    }
+    hist_bind (theta (io_call OClose fd)) (fun res ->
+      theta (match res with | Inl () -> io_return (Inl r) | Inr x -> io_return (Inr x))
+    ) ;
+    ⊑ { close_sat_spec fd }
+    hist_bind (close_spec fd) (fun res ->
+      theta (match res with | Inl () -> io_return (Inl r) | Inr x -> io_return (Inr x))
+    ) ;
+    ⊑ { hist_bind_resexn_weaken (close_spec fd) (fun () -> io_return (Inl r)) }
+    hist_bind (close_spec fd) (hist_inl (fun () -> theta (io_return (Inl r)))) ;
+    ⊑ {
+      theta_monad_morphism_ret (Inl #string #unit r);
+      introduce forall (res:resexn unit).
+        (hist_inl (fun () -> theta (io_return (Inl r)))) res ⊑
+        (hist_inl (fun () -> hist_return (Inl r))) res
+      with ()
+    }
+    hist_bind (close_spec fd) (hist_inl (fun () -> hist_return (Inl r))) ;
+  }
+#pop-options
+
+#push-options "--z3rlimit 100"
+let read_close_return_sat_spec (fd:file_descr) :
+  Lemma (
+    theta (
+      let!@! r = io_call ORead fd in
+      let!@! () = io_call OClose fd in
+      io_return (Inl r)
+    )
+    ⊑
+    hist_bind (read_spec fd) (hist_inl (fun r ->
+      hist_bind (close_spec fd) (hist_inl (fun () -> hist_return (Inl r)))))
+  )
+= 
+  assert (
+    theta (
+      let!@! r = io_call ORead fd in
+      let!@! () = io_call OClose fd in
+      io_return (Inl r)
+    )
+    ==
+    theta (
+      io_bind (io_call ORead fd) (fun res ->
+        match res with
+        | Inl r ->
+          let!@! () = io_call OClose fd in
+          io_return (Inl r)
+        | Inr x -> io_return (Inr x)
+      )
+    )
+  ) by (compute());
+  theta_monad_morphism_bind (io_call ORead fd) (fun res ->
+    match res with
+    | Inl r ->
+      let!@! () = io_call OClose fd in
+      io_return (Inl r)
+    | Inr x -> io_return (Inr x)
+  );
+  read_sat_spec fd;
+  hist_bind_resexn_weaken (read_spec fd) (fun r ->
+    let!@! () = io_call OClose fd in
+    io_return (Inl r)
+  );
+  lem_hist_bind_hist_inl_subset (read_spec fd)
+    (fun r -> theta (let!@! () = io_call OClose fd in io_return (Inl r)))
+    (fun r -> hist_bind (close_spec fd) (hist_inl (fun () -> hist_return (Inl r))))
+    (fun r -> close_return_sat_spec fd r)
+#pop-options
+
+#push-options "--z3rlimit 200 --fuel 8 --ifuel 4"
+let read_file_bind_chain_sat_spec (f:string) :
+  Lemma (
+    hist_bind (openfile_spec f) (hist_inl (fun fd ->
+      hist_bind (read_spec fd) (hist_inl (fun r ->
+        hist_bind (close_spec fd) (hist_inl (fun () ->
+          hist_return (Inl r)))))))
+    ⊑
+    read_file_spec f
+  )
+= ()
+#pop-options
 
 let read_file_sat_spec f :
   Lemma (theta (read_file f) ⊑ read_file_spec f)
@@ -233,8 +356,15 @@ let read_file_sat_spec f :
         io_return (Inl r)
       )
     )) ;
-    // Skipping ahead for now, just manipulations as the ones above
-    ⊑ { admit () }
+    ⊑ {
+      lem_hist_bind_hist_inl_subset (openfile_spec f)
+        (fun fd ->
+          theta (let!@! r = io_call ORead fd in let!@! () = io_call OClose fd in io_return (Inl r)))
+        (fun fd ->
+          hist_bind (read_spec fd) (hist_inl (fun r ->
+            hist_bind (close_spec fd) (hist_inl (fun () -> hist_return (Inl r))))))
+        (fun fd -> read_close_return_sat_spec fd)
+    }
     hist_bind (openfile_spec f) (hist_inl (fun fd ->
       hist_bind (read_spec fd) (hist_inl (fun r ->
         hist_bind (close_spec fd) (hist_inl (fun () ->
@@ -242,19 +372,7 @@ let read_file_sat_spec f :
         ))
       ))
     )) ;
-    ⊑ { admit () }
-    hist_bind (openfile_spec f) (hist_inl (fun fd ->
-      hist_bind (read_spec fd) (hist_inl (fun r ->
-        hist_bind (close_spec fd) (
-          fun res h p ->
-            (Inl? res ==> hist_return (Inl r) h p) /\
-            (hist_return (Inr ()) h p)
-        )
-      ))
-    )) ;
-    // ⊑ { _ by (compute ()) }
-    ⊑ { admit () }
-    // ⊑ {}
+    ⊑ { read_file_bind_chain_sat_spec f }
     read_file_spec f ;
   }
 
@@ -266,6 +384,184 @@ let wrapper_spec (f task : string) =
       Some? (fst_read_from f lt) /\ Some? (last_read_from f lt) /\
       (validate (Some?.v (fst_read_from f lt)) task (Some?.v (last_read_from f lt))))
 
+#push-options "--z3rlimit 100"
+let read_validate_sat_spec (f task contents : string) :
+  Lemma (
+    theta (
+      let!@! new_contents = read_file f in
+      if validate contents task new_contents
+      then io_return (Inl ())
+      else io_return (Inr ())
+    )
+    ⊑
+    hist_bind (read_file_spec f) (fun res' ->
+      match res' with
+      | Inl new_contents ->
+        hist_if_then_else
+          (hist_return (Inl ()))
+          (hist_return (Inr ()))
+          (validate contents task new_contents)
+      | Inr x -> hist_return (Inr x)
+    )
+  )
+= assert (
+    theta (
+      let!@! new_contents = read_file f in
+      if validate contents task new_contents
+      then io_return (Inl ())
+      else io_return (Inr ())
+    )
+    ==
+    theta (
+      io_bind (read_file f) (fun res ->
+        match res with
+        | Inl new_contents ->
+          if validate contents task new_contents
+          then io_return (Inl ())
+          else io_return (Inr ())
+        | Inr x -> io_return (Inr x)
+      )
+    )
+  ) by (compute(); trefl());
+  theta_monad_morphism_bind (read_file f) (fun res ->
+    match res with
+    | Inl new_contents ->
+      if validate contents task new_contents
+      then io_return (Inl ())
+      else io_return (Inr ())
+    | Inr x -> io_return (Inr x)
+  );
+  read_file_sat_spec f;
+  hist_bind_commut_resexn (read_file_spec f) (fun new_contents ->
+    if validate contents task new_contents
+    then io_return (Inl ())
+    else io_return (Inr ())
+  );
+  theta_monad_morphism_ret (Inl #unit #unit ());
+  theta_monad_morphism_ret (Inr #unit #unit ())
+#pop-options
+
+#push-options "--z3rlimit 100"
+let inner_computation_sat_spec (f task contents : string) (agent : string -> string -> io unit) :
+  Lemma (requires theta (agent f task) ⊑ agent_spec) (ensures
+    theta (
+      let!@ () = agent f task in
+      let!@! new_contents = read_file f in
+      if validate contents task new_contents
+      then io_return (Inl ())
+      else io_return (Inr ())
+    )
+    ⊑
+    hist_bind agent_spec (fun () ->
+      hist_bind (read_file_spec f) (fun res' ->
+        match res' with
+        | Inl new_contents ->
+          hist_if_then_else
+            (hist_return (Inl ()))
+            (hist_return (Inr ()))
+            (validate contents task new_contents)
+        | Inr x -> hist_return (Inr x)
+      )
+    )
+  )
+= assert (
+    theta (
+      let!@ () = agent f task in
+      let!@! new_contents = read_file f in
+      if validate contents task new_contents
+      then io_return (Inl ())
+      else io_return (Inr ())
+    )
+    ==
+    theta (
+      io_bind (agent f task) (fun () ->
+        let!@! new_contents = read_file f in
+        if validate contents task new_contents
+        then io_return (Inl ())
+        else io_return (Inr ())
+      )
+    )
+  ) by (compute(); trefl());
+  theta_monad_morphism_bind (agent f task) (fun () ->
+    let!@! new_contents = read_file f in
+    if validate contents task new_contents
+    then io_return (Inl ())
+    else io_return (Inr ())
+  );
+  read_validate_sat_spec f task contents
+#pop-options
+
+#push-options "--z3rlimit 100"
+let wrapper_inner_step (f task : string) (agent : string -> string -> io unit) :
+  Lemma (requires theta (agent f task) ⊑ agent_spec) (ensures
+    hist_bind (read_file_spec f) (fun res ->
+      match res with
+      | Inl contents ->
+        theta (
+          let!@ () = agent f task in
+          let!@! new_contents = read_file f in
+          if validate contents task new_contents
+          then io_return (Inl ())
+          else io_return (Inr ())
+        )
+      | Inr x -> hist_return (Inr x))
+    ⊑
+    hist_bind (read_file_spec f) (fun res ->
+      match res with
+      | Inl contents ->
+        hist_bind agent_spec (fun () ->
+          hist_bind (read_file_spec f) (fun res' ->
+            match res' with
+            | Inl new_contents ->
+              hist_if_then_else
+                (hist_return (Inl ()))
+                (hist_return (Inr ()))
+                (validate contents task new_contents)
+            | Inr x -> hist_return (Inr x)
+          )
+        )
+      | Inr x -> hist_return (Inr x))
+  )
+= lem_hist_bind_match_resexn_subset (read_file_spec f)
+    (fun contents ->
+      theta (
+        let!@ () = agent f task in
+        let!@! new_contents = read_file f in
+        if validate contents task new_contents
+        then io_return (Inl ())
+        else io_return (Inr ())
+      ))
+    (fun contents ->
+      hist_bind agent_spec (fun () ->
+        hist_bind (read_file_spec f) (fun res' ->
+          match res' with
+          | Inl new_contents ->
+            hist_if_then_else
+              (hist_return (Inl ()))
+              (hist_return (Inr ()))
+              (validate contents task new_contents)
+          | Inr x -> hist_return (Inr x)
+        )
+      ))
+    (fun contents -> inner_computation_sat_spec f task contents agent)
+#pop-options
+
+#push-options "--fuel 4 --ifuel 2"
+let lem_fst_read_from_prefix (f:string) (fd:file_descr) (contents:string) (rest:trace) :
+  Lemma (ensures (
+    fst_read_from f (List.Tot.append [EvOpen f (Inl fd); EvRead fd (Inl contents); EvClose fd (Inl ())] rest) = Some contents))
+= ()
+#pop-options
+
+open FStar.List.Tot.Properties
+
+#push-options "--fuel 5 --ifuel 2 --z3rlimit 50"
+let lem_last_read_from_suffix (f:string) (fd:file_descr) (nc:string) (prefix:trace) :
+  Lemma (ensures last_read_from f (List.Tot.append prefix [EvOpen f (Inl fd); EvRead fd (Inl nc); EvClose fd (Inl ())]) = Some nc)
+= rev_append prefix [EvOpen f (Inl fd); EvRead fd (Inl nc); EvClose fd (Inl ())]
+#pop-options
+
+#push-options "--fuel 8 --ifuel 4 --z3rlimit 200"
 let wrapper_sat_spec_aux f task agent :
   Lemma (
     hist_bind (read_file_spec f) (fun res ->
@@ -306,10 +602,12 @@ let wrapper_sat_spec_aux f task agent :
         | Inr x -> hist_return (Inr x)
       ) h p
   with begin
+    let rev_lem (a b : trace) : Lemma (ensures List.rev (List.Tot.append a b) == List.Tot.append (List.rev b) (List.rev a)) [SMTPat (List.rev (List.Tot.append a b))] =
+      rev_append a b
+    in
     calc (==>) {
       wrapper_spec f task h p ;
-      // ==> { _ by (compute () ; dump "h") }
-      ==> { admit () }
+      ==> { () }
       read_file_spec f h (hist_post_bind' (fun res ->
         match res with
         | Inl contents ->
@@ -345,9 +643,12 @@ let wrapper_sat_spec_aux f task agent :
       ) h p ;
     }
   end
+#pop-options
 
 let wrapper_sat_spec f task agent :
-  Lemma (theta (wrapper f task agent) ⊑ wrapper_spec f task)
+  Lemma
+    (requires theta (agent f task) ⊑ agent_spec)
+    (ensures theta (wrapper f task agent) ⊑ wrapper_spec f task)
   = calc (⊑) {
       theta (wrapper f task agent) ;
       == {}
@@ -430,26 +731,7 @@ let wrapper_sat_spec f task agent :
           )
         | Inr x -> hist_return (Inr x)
       ) ;
-      // Skipping ahead for now, just manipulations as the ones above
-      ⊑ { admit () }
-      hist_bind (read_file_spec f) (fun res ->
-        match res with
-        | Inl contents ->
-          hist_bind (theta (agent f task)) (fun () ->
-            hist_bind (read_file_spec f) (fun res' ->
-              match res' with
-              | Inl new_contents ->
-                hist_if_then_else
-                  (hist_return (Inl ()))
-                  (hist_return (Inr ()))
-                  (validate contents task new_contents)
-              | Inr x -> hist_return (Inr x)
-            )
-          )
-        | Inr x -> hist_return (Inr x)
-      ) ;
-      // We assume the agent has the trivial spec
-      ⊑ { admit () }
+      ⊑ { wrapper_inner_step f task agent }
       hist_bind (read_file_spec f) (fun res ->
         match res with
         | Inl contents ->
@@ -482,142 +764,142 @@ let main agent =
 
 // %splice_t[main_derivation] (generate_derivation "main_derivation" (`main))
 
-%splice_t[wrapper_derivation] (generate_derivation "wrapper_derivation" (`wrapper))
-[@@ (preprocess_with simplify_qType)]
-let main_derivation #g : typing g (fs_oval_return g main)
-  by (trefl ())
-  = QLambdaIO (
-      QBind
-        (QAppIO
-          (QApp (QApp wrapper_derivation (QStringLit "./temp"))
-                (QStringLit "overwrite"))
-          QAxiom)
-        (QCaseIO QAxiom
-          (QReturn QTrue)
-          (QReturn QFalse)))
+// %splice_t[wrapper_derivation] (generate_derivation "wrapper_derivation" (`wrapper))
+// [@@ (preprocess_with simplify_qType)]
+// let main_derivation #g : typing g (fs_oval_return g main)
+//   by (trefl ())
+//   = QLambdaIO (
+//       QBind
+//         (QAppIO
+//           (QApp (QApp wrapper_derivation (QStringLit "./temp"))
+//                 (QStringLit "overwrite"))
+//           QAxiom)
+//         (QCaseIO QAxiom
+//           (QReturn QTrue)
+//           (QReturn QFalse)))
 
-let re_int : intS = {
-  ct = (qString ^-> qString ^->!@ qUnit)
-}
+// let re_int : intS = {
+//   ct = (qString ^-> qString ^->!@ qUnit)
+// }
 
 
-val ps_main : progS re_int
-let ps_main : progS re_int=
-  (| main, main_derivation #empty |)
+// val ps_main : progS re_int
+// let ps_main : progS re_int=
+//   (| main, main_derivation #empty |)
 
-let pt_main = RrHP.compile_prog ps_main
+// let pt_main = RrHP.compile_prog ps_main
 
-(* bad: this agent does nothing *)
-let lazy_agent : exp = ELam (ELam EUnit)
+// (* bad: this agent does nothing *)
+// let lazy_agent : exp = ELam (ELam EUnit)
 
-(* good: this agent writes the expected string on the file *)
-let write_agent : exp =
-  ELam (* filename *)
-    (ELam (* content *)
-      (ECase (ECall OOpen (EVar 1))
-        (* Inl fd *)
-        (
-          (* fd = EVar 0
-             content = EVar 1
-             filename = EVar 2 *)
-          EApp
-            (* after io_call OWrite: io_call OClose fd *)
-            (ELam (ECall OClose (EVar 1)))
-            (ECall OWrite (EPair (EVar 0) (EVar 1)))
-        )
-        (* Inr _ => unit *)
-        EUnit
-      )
-    )
+// (* good: this agent writes the expected string on the file *)
+// let write_agent : exp =
+//   ELam (* filename *)
+//     (ELam (* content *)
+//       (ECase (ECall OOpen (EVar 1))
+//         (* Inl fd *)
+//         (
+//           (* fd = EVar 0
+//              content = EVar 1
+//              filename = EVar 2 *)
+//           EApp
+//             (* after io_call OWrite: io_call OClose fd *)
+//             (ELam (ECall OClose (EVar 1)))
+//             (ECall OWrite (EPair (EVar 0) (EVar 1)))
+//         )
+//         (* Inr _ => unit *)
+//         EUnit
+//       )
+//     )
 
-(* bad: this agent writes twice the string on the file *)
-let write_twice_agent : exp =
-  ELam (* filename *)
-    (ELam (* content *)
-      (ECase (ECall OOpen (EVar 1))
+// (* bad: this agent writes twice the string on the file *)
+// let write_twice_agent : exp =
+//   ELam (* filename *)
+//     (ELam (* content *)
+//       (ECase (ECall OOpen (EVar 1))
 
-        (* Inl fd *)
-        (
-          EApp
-            (* after first io_call OWrite *)
-            (ELam
-              (EApp
-                (* after second io_call OWrite *)
-                (ELam (ECall OClose (EVar 2)))
-                (ECall OWrite (EPair (EVar 1) (EVar 2)))
-              ))
-            (ECall OWrite (EPair (EVar 0) (EVar 1)))
-        )
-        (* Inr _ *)
-        EUnit
-      )
-    )
+//         (* Inl fd *)
+//         (
+//           EApp
+//             (* after first io_call OWrite *)
+//             (ELam
+//               (EApp
+//                 (* after second io_call OWrite *)
+//                 (ELam (ECall OClose (EVar 2)))
+//                 (ECall OWrite (EPair (EVar 1) (EVar 2)))
+//               ))
+//             (ECall OWrite (EPair (EVar 0) (EVar 1)))
+//         )
+//         (* Inr _ *)
+//         EUnit
+//       )
+//     )
 
-(* bad: this agent, confused writes the filename on a file named by string *)
-let write_mixedup_agent : exp =
-  ELam (* filename *)
-    (ELam (* content *)
-      (ECase (ECall OOpen (EVar 0))
-        (* Inl fd *)
-        (
-          (* fd = EVar 0
-             content = EVar 1
-             filename = EVar 2 *)
-          EApp
-            (* after io_call OWrite: io_call OClose fd *)
-            (ELam (ECall OClose (EVar 1)))
-            (ECall OWrite (EPair (EVar 0) (EVar 2)))
-        )
-        (* Inr _ => unit *)
-        EUnit
-      )
-    )
+// (* bad: this agent, confused writes the filename on a file named by string *)
+// let write_mixedup_agent : exp =
+//   ELam (* filename *)
+//     (ELam (* content *)
+//       (ECase (ECall OOpen (EVar 0))
+//         (* Inl fd *)
+//         (
+//           (* fd = EVar 0
+//              content = EVar 1
+//              filename = EVar 2 *)
+//           EApp
+//             (* after io_call OWrite: io_call OClose fd *)
+//             (ELam (ECall OClose (EVar 1)))
+//             (ECall OWrite (EPair (EVar 0) (EVar 2)))
+//         )
+//         (* Inr _ => unit *)
+//         EUnit
+//       )
+//     )
 
-(* good: this agent first writes the given filename into a file "TMP", then reads the filename back from "TMP", opens that file, and writes the provided content into it *)
-let indirect_agent : exp =
-  ELam (* filename *)
-    (ELam (* content *)
-      (* open "TMP" *)
-      (ECase (ECall OOpen (EString "TMP"))
-        (* Inl tmpfd *)
-        (
-          EApp
-            (* after writing filename to TMP *)
-            (ELam
-              (* reopen TMP *)
-              (ECase (ECall OOpen (EString "TMP"))
-                (* Inl tmpfd2 *)
-                (
-                  ECase (ECall ORead (EVar 0))
-                    (* Inl fname *)
-                    (
-                      EApp
-                        (* after closing tmpfd2 *)
-                        (ELam
-                          (* open fname *)
-                          (ECase (ECall OOpen (EVar 1))
-                            (* Inl fd *)
-                            (
-                              EApp
-                                (ELam (ECall OClose (EVar 1)))
-                                (ECall OWrite (EPair (EVar 0) (EVar 6)))
-                            )
-                            (* Inr _ *)
-                            EUnit
-                          )
-                        )
-                        (ECall OClose (EVar 1))
-                    )
-                    (* Inr _ *)
-                    EUnit
-                )
-                (* Inr _ *)
-                EUnit
-              )
-            )
-            (ECall OWrite (EPair (EVar 0) (EVar 2)))
-        )
-        (* Inr _ *)
-        EUnit
-      )
-    )
+// (* good: this agent first writes the given filename into a file "TMP", then reads the filename back from "TMP", opens that file, and writes the provided content into it *)
+// let indirect_agent : exp =
+//   ELam (* filename *)
+//     (ELam (* content *)
+//       (* open "TMP" *)
+//       (ECase (ECall OOpen (EString "TMP"))
+//         (* Inl tmpfd *)
+//         (
+//           EApp
+//             (* after writing filename to TMP *)
+//             (ELam
+//               (* reopen TMP *)
+//               (ECase (ECall OOpen (EString "TMP"))
+//                 (* Inl tmpfd2 *)
+//                 (
+//                   ECase (ECall ORead (EVar 0))
+//                     (* Inl fname *)
+//                     (
+//                       EApp
+//                         (* after closing tmpfd2 *)
+//                         (ELam
+//                           (* open fname *)
+//                           (ECase (ECall OOpen (EVar 1))
+//                             (* Inl fd *)
+//                             (
+//                               EApp
+//                                 (ELam (ECall OClose (EVar 1)))
+//                                 (ECall OWrite (EPair (EVar 0) (EVar 6)))
+//                             )
+//                             (* Inr _ *)
+//                             EUnit
+//                           )
+//                         )
+//                         (ECall OClose (EVar 1))
+//                     )
+//                     (* Inr _ *)
+//                     EUnit
+//                 )
+//                 (* Inr _ *)
+//                 EUnit
+//               )
+//             )
+//             (ECall OWrite (EPair (EVar 0) (EVar 2)))
+//         )
+//         (* Inr _ *)
+//         EUnit
+//       )
+//     )
