seiostar/sandbox.entrypoint.sh
@@ -6,7 +6,7 @@ git config --global --add safe.directory /workspace
 git config --global user.email "cezar.andrici@gmail.com"
 git config --global user.name "Cezar Andrici"
 
-echo "alias mycc='make verify -j 8 && claude --dangerously-skip-permissions'" > ~/.bashrc
-echo "alias myco='make verify -j 8 && copilot --yolo'" > ~/.bashrc
+echo "alias mycc='make verify -j 8; claude --dangerously-skip-permissions'" > ~/.bashrc
+echo "alias myco='make verify -j 8; copilot --yolo --model claude-opus-4.6'" > ~/.bashrc
 
 exec "$@"
